add cmp spec and verify compare_int

examples/binary_search.c
@@ -3,11 +3,11 @@
 
 // compiled with armv8-a clang 11.0.1
 // options: -O2
-// https://godbolt.org/z/sEGvPoPox
+// https://godbolt.org/z/rzaGjecGK
 
-typedef bool (*comp_fn)(void *, void *);
+typedef bool (*comp_fn)(size_t, size_t);
 
-size_t binary_search(comp_fn comp, void **xs, size_t n, void *x) {
+size_t binary_search(comp_fn comp, size_t *xs, size_t n, size_t x) {
   size_t l = 0, r = n;
   while(l < r) {
     size_t k = l + (r - l) / 2;
@@ -20,7 +20,7 @@ size_t binary_search(comp_fn comp, void **xs, size_t n, void *x) {
   return l;
 }
 
-bool compare_int(void *x, void *y) {
-  size_t *xi = x, *yi = y;
-  return *xi <= *yi;
+
+bool compare_int(size_t x, size_t y) {
+  return x <= y;
 }
