instructions/binary_search/a74.v
@@ -2,35 +2,30 @@ From isla Require Import isla_lang.
 
 Definition a74 : list trc := [
   [
-    Smt (DeclareConst 6%Z (Ty_BitVec 1%N)) Mk_annot;
-    Smt (DeclareConst 29%Z (Ty_BitVec 64%N)) Mk_annot;
-    Smt (Assert (Binop (Eq) (Manyop (Bvmanyarith Bvand) [Val (Val_Symbolic 29%Z) Mk_annot; Val (Val_Bits [BV{64%N} 0xfff0000000000007%Z]) Mk_annot] Mk_annot) (Val (Val_Bits [BV{64%N} 0x0%Z]) Mk_annot) Mk_annot)) Mk_annot;
-    ReadReg "R0" [] (RegVal_Base (Val_Symbolic 29%Z)) Mk_annot;
-    Smt (DefineConst 90%Z (Manyop (Bvmanyarith Bvadd) [Val (Val_Symbolic 29%Z) Mk_annot; Val (Val_Bits [BV{64%N} 0x0%Z]) Mk_annot] Mk_annot)) Mk_annot;
-    ReadReg "PSTATE" [Field "EL"] (RegVal_Struct [("EL", RegVal_Base (Val_Bits [BV{2%N} 0x2%Z]))]) Mk_annot;
-    Smt (DefineConst 94%Z (Binop (Eq) (Val (Val_Symbolic 90%Z) Mk_annot) (Manyop (Bvmanyarith Bvand) [Val (Val_Symbolic 90%Z) Mk_annot; Val (Val_Bits [BV{64%N} 0xfffffffffffffff8%Z]) Mk_annot] Mk_annot) Mk_annot)) Mk_annot;
-    ReadReg "SCTLR_EL2" [] (RegVal_Base (Val_Bits [BV{64%N} 0x4000002%Z])) Mk_annot;
-    Smt (Assert (Unop (Not) (Unop (Not) (Val (Val_Symbolic 94%Z) Mk_annot) Mk_annot) Mk_annot)) Mk_annot;
-    Smt (Assert (Unop (Not) (Unop (Not) (Val (Val_Symbolic 94%Z) Mk_annot) Mk_annot) Mk_annot)) Mk_annot;
-    Smt (Assert (Binop (Eq) (Val (Val_Symbolic 90%Z) Mk_annot) (Manyop (Bvmanyarith Bvand) [Val (Val_Symbolic 90%Z) Mk_annot; Val (Val_Bits [BV{64%N} 0xfffffffffffffff8%Z]) Mk_annot] Mk_annot) Mk_annot)) Mk_annot;
-    ReadReg "CFG_ID_AA64PFR0_EL1_EL2" [] (RegVal_Base (Val_Bits [BV{4%N} 0x1%Z])) Mk_annot;
-    ReadReg "CFG_ID_AA64PFR0_EL1_EL3" [] (RegVal_Base (Val_Bits [BV{4%N} 0x1%Z])) Mk_annot;
-    ReadReg "PSTATE" [Field "nRW"] (RegVal_Struct [("nRW", RegVal_Base (Val_Bits [BV{1%N} 0x0%Z]))]) Mk_annot;
-    ReadReg "CFG_ID_AA64PFR0_EL1_EL0" [] (RegVal_Base (Val_Bits [BV{4%N} 0x1%Z])) Mk_annot;
-    ReadReg "CFG_ID_AA64PFR0_EL1_EL1" [] (RegVal_Base (Val_Bits [BV{4%N} 0x1%Z])) Mk_annot;
-    ReadReg "SCR_EL3" [] (RegVal_Base (Val_Bits [BV{32%N} 0x0%Z])) Mk_annot;
-    ReadReg "TCR_EL2" [] (RegVal_Base (Val_Bits [BV{64%N} 0x0%Z])) Mk_annot;
-    Smt (Assert (Unop (Not) (Unop (Not) (Binop (Eq) (Unop (Extract 63%N 52%N) (Val (Val_Symbolic 90%Z) Mk_annot) Mk_annot) (Val (Val_Bits [BV{12%N} 0x0%Z]) Mk_annot) Mk_annot) Mk_annot) Mk_annot)) Mk_annot;
-    Smt (Assert (Unop (Not) (Unop (Not) (Val (Val_Symbolic 94%Z) Mk_annot) Mk_annot) Mk_annot)) Mk_annot;
-    ReadReg "PSTATE" [Field "D"] (RegVal_Struct [("D", RegVal_Base (Val_Symbolic 6%Z))]) Mk_annot;
-    ReadReg "OSLSR_EL1" [] (RegVal_Base (Val_Bits [BV{32%N} 0x0%Z])) Mk_annot;
-    ReadReg "OSDLR_EL1" [] (RegVal_Base (Val_Bits [BV{32%N} 0x0%Z])) Mk_annot;
-    ReadReg "EDSCR" [] (RegVal_Base (Val_Bits [BV{32%N} 0x0%Z])) Mk_annot;
-    Smt (DeclareConst 1280%Z (Ty_BitVec 56%N)) Mk_annot;
-    Smt (DefineConst 1289%Z (Unop (ZeroExtend 8%N) (Manyop Concat [Val (Val_Bits [BV{4%N} 0x0%Z]) Mk_annot; Unop (Extract 51%N 0%N) (Val (Val_Symbolic 90%Z) Mk_annot) Mk_annot] Mk_annot) Mk_annot)) Mk_annot;
-    Smt (DeclareConst 1290%Z (Ty_BitVec 64%N)) Mk_annot;
-    ReadMem (RegVal_Base (Val_Symbolic 1290%Z)) (RegVal_Base (Val_Enum ((Mk_enum_id 6%nat), Mk_enum_ctor 0%nat))) (RegVal_Base (Val_Symbolic 1289%Z)) 8%N None Mk_annot;
-    Smt (DefineConst 1294%Z (Val (Val_Symbolic 1290%Z) Mk_annot)) Mk_annot;
-    WriteReg "R8" [] (RegVal_Base (Val_Symbolic 1294%Z)) Mk_annot
+    Smt (DeclareConst 5%Z (Ty_BitVec 1%N)) Mk_annot;
+    Smt (DeclareConst 17%Z (Ty_BitVec 1%N)) Mk_annot;
+    Smt (DeclareConst 26%Z (Ty_BitVec 1%N)) Mk_annot;
+    Smt (DeclareConst 27%Z (Ty_BitVec 1%N)) Mk_annot;
+    Smt (DeclareConst 42%Z (Ty_BitVec 64%N)) Mk_annot;
+    ReadReg "R0" [] (RegVal_Base (Val_Symbolic 42%Z)) Mk_annot;
+    Smt (DefineConst 43%Z (Val (Val_Symbolic 42%Z) Mk_annot)) Mk_annot;
+    Smt (DeclareConst 44%Z (Ty_BitVec 64%N)) Mk_annot;
+    ReadReg "R1" [] (RegVal_Base (Val_Symbolic 44%Z)) Mk_annot;
+    Smt (DefineConst 50%Z (Unop (Bvnot) (Val (Val_Symbolic 44%Z) Mk_annot) Mk_annot)) Mk_annot;
+    Smt (DefineConst 54%Z (Manyop (Bvmanyarith Bvadd) [Manyop (Bvmanyarith Bvadd) [Unop (ZeroExtend 64%N) (Val (Val_Symbolic 43%Z) Mk_annot) Mk_annot; Unop (ZeroExtend 64%N) (Val (Val_Symbolic 50%Z) Mk_annot) Mk_annot] Mk_annot; Val (Val_Bits [BV{128%N} 0x1%Z]) Mk_annot] Mk_annot)) Mk_annot;
+    Smt (DefineConst 59%Z (Unop (Extract 63%N 0%N) (Val (Val_Symbolic 54%Z) Mk_annot) Mk_annot)) Mk_annot;
+    Smt (DefineConst 72%Z (Manyop Concat [Manyop Concat [Manyop Concat [Manyop (Bvmanyarith Bvor) [Manyop (Bvmanyarith Bvand) [Val (Val_Bits [BV{1%N} 0x0%Z]) Mk_annot; Unop (Bvnot) (Val (Val_Bits [BV{1%N} 0x1%Z]) Mk_annot) Mk_annot] Mk_annot; Unop (Extract 0%N 0%N) (Binop ((Bvarith Bvlshr)) (Val (Val_Symbolic 59%Z) Mk_annot) (Unop (Extract 63%N 0%N) (Val (Val_Bits [BV{128%N} 0x3f%Z]) Mk_annot) Mk_annot) Mk_annot) Mk_annot] Mk_annot; Ite (Binop (Eq) (Val (Val_Symbolic 59%Z) Mk_annot) (Val (Val_Bits [BV{64%N} 0x0%Z]) Mk_annot) Mk_annot) (Val (Val_Bits [BV{1%N} 0x1%Z]) Mk_annot) (Val (Val_Bits [BV{1%N} 0x0%Z]) Mk_annot) Mk_annot] Mk_annot; Ite (Binop (Eq) (Unop (ZeroExtend 64%N) (Val (Val_Symbolic 59%Z) Mk_annot) Mk_annot) (Val (Val_Symbolic 54%Z) Mk_annot) Mk_annot) (Val (Val_Bits [BV{1%N} 0x0%Z]) Mk_annot) (Val (Val_Bits [BV{1%N} 0x1%Z]) Mk_annot) Mk_annot] Mk_annot; Ite (Binop (Eq) (Unop (SignExtend 64%N) (Val (Val_Symbolic 59%Z) Mk_annot) Mk_annot) (Manyop (Bvmanyarith Bvadd) [Manyop (Bvmanyarith Bvadd) [Unop (SignExtend 64%N) (Val (Val_Symbolic 43%Z) Mk_annot) Mk_annot; Unop (SignExtend 64%N) (Val (Val_Symbolic 50%Z) Mk_annot) Mk_annot] Mk_annot; Val (Val_Bits [BV{128%N} 0x1%Z]) Mk_annot] Mk_annot) Mk_annot) (Val (Val_Bits [BV{1%N} 0x0%Z]) Mk_annot) (Val (Val_Bits [BV{1%N} 0x1%Z]) Mk_annot) Mk_annot] Mk_annot)) Mk_annot;
+    Smt (DefineConst 74%Z (Unop (Extract 3%N 3%N) (Val (Val_Symbolic 72%Z) Mk_annot) Mk_annot)) Mk_annot;
+    ReadReg "PSTATE" [Field "N"] (RegVal_Struct [("N", RegVal_Base (Val_Symbolic 17%Z))]) Mk_annot;
+    WriteReg "PSTATE" [Field "N"] (RegVal_Struct [("N", RegVal_Base (Val_Symbolic 74%Z))]) Mk_annot;
+    Smt (DefineConst 75%Z (Unop (Extract 2%N 2%N) (Val (Val_Symbolic 72%Z) Mk_annot) Mk_annot)) Mk_annot;
+    ReadReg "PSTATE" [Field "Z"] (RegVal_Struct [("Z", RegVal_Base (Val_Symbolic 27%Z))]) Mk_annot;
+    WriteReg "PSTATE" [Field "Z"] (RegVal_Struct [("Z", RegVal_Base (Val_Symbolic 75%Z))]) Mk_annot;
+    Smt (DefineConst 76%Z (Unop (Extract 1%N 1%N) (Val (Val_Symbolic 72%Z) Mk_annot) Mk_annot)) Mk_annot;
+    ReadReg "PSTATE" [Field "C"] (RegVal_Struct [("C", RegVal_Base (Val_Symbolic 5%Z))]) Mk_annot;
+    WriteReg "PSTATE" [Field "C"] (RegVal_Struct [("C", RegVal_Base (Val_Symbolic 76%Z))]) Mk_annot;
+    Smt (DefineConst 77%Z (Unop (Extract 0%N 0%N) (Val (Val_Symbolic 72%Z) Mk_annot) Mk_annot)) Mk_annot;
+    ReadReg "PSTATE" [Field "V"] (RegVal_Struct [("V", RegVal_Base (Val_Symbolic 26%Z))]) Mk_annot;
+    WriteReg "PSTATE" [Field "V"] (RegVal_Struct [("V", RegVal_Base (Val_Symbolic 77%Z))]) Mk_annot
   ]
 ].
