instructions/binary_search/a4c_spec.v
@@ -1,0 +1,15 @@
+Require Import isla.isla.
+Require Export isla.instructions.binary_search.a4c.
+
+Lemma a4c_spec `{!islaG Σ} `{!threadG}:
+  instr 0x1030004c (Some a4c) -∗
+  instr_body 0x1030004c (cmp_R_R_spec 0x000000001030004c "R20" "R23").
+Proof.
+  iStartProof.
+  repeat liAStep; liShow.
+  Unshelve. all: prepare_sidecond.
+  1: cmp_spec_tac1. 1: cmp_spec_tac2. 1: cmp_spec_tac3. 1: cmp_spec_tac4.
+Qed.
+
+Definition a4c_spec_inst `{!islaG Σ} `{!threadG} := entails_to_simplify_hyp 0 a4c_spec.
+Global Existing Instance a4c_spec_inst.
