instructions/binary_search/a74_spec.v
@@ -1,0 +1,15 @@
+Require Import isla.isla.
+Require Export isla.instructions.binary_search.a74.
+
+Lemma a74_spec `{!islaG Σ} `{!threadG}:
+  instr 0x10300074 (Some a74) -∗
+  instr_body 0x10300074 (cmp_R_R_spec 0x0000000010300074 "R0" "R1").
+Proof.
+  iStartProof.
+  repeat liAStep; liShow.
+  Unshelve. all: prepare_sidecond.
+  1: cmp_spec_tac1. 1: cmp_spec_tac2. 1: cmp_spec_tac3. 1: cmp_spec_tac4.
+Qed.
+
+Definition a74_spec_inst `{!islaG Σ} `{!threadG} := entails_to_simplify_hyp 0 a74_spec.
+Global Existing Instance a74_spec_inst.
